NOT BUILDING: fixed overall proof for new Ifun strategy, AC kernel proof still missing

integrityScript.sml
@@ -12,13 +12,13 @@ val _ = new_theory "integrity";
 (******** import Inv interface ********)
 
 val CR_lem = store_thm("CR_lem", ``
-!s s'. (!r. r IN CR s ==> (Cv s r = Cv s' r)) ==> (CR s = CR s')
+!s s'. Ifun s /\ (!r. r IN CR s ==> (Cv s r = Cv s' r)) ==> (CR s = CR s')
 ``,
   REWRITE_TAC [CR_oblg]
 );
 
 val CR_coreg_lem = store_thm("CR_coreg_lem", ``
-!s s' r. reg_res r /\ r IN CR s /\ (s'.cs.coreg = s.cs.coreg) ==> 
+!s s' r. Ifun s /\ reg_res r /\ r IN CR s /\ (s'.cs.coreg = s.cs.coreg) ==> 
     (Cv s r = Cv s' r) 
 ``,
   REWRITE_TAC [CR_coreg_oblg]
@@ -58,6 +58,7 @@ val Ifun_Mon_lem = store_thm("Ifun_Mon_lem", ``
 val Icoh_CR_lem = store_thm("Icoh_CR_lem", ``
 !s s' Icoh Icode Icm.
        cm_user_po Icoh Icode Icm  
+    /\ Ifun s
     /\ dCoh s.ms {pa | MEM pa IN CR s} 
     /\ dCoh s'.ms {pa | MEM pa IN CR s'}
     /\ (!r. r IN CR s ==> (Cv s r = Cv s' r))
@@ -68,7 +69,7 @@ val Icoh_CR_lem = store_thm("Icoh_CR_lem", ``
 ); 
 
 val Icoh_dCoh_lem = store_thm("Icoh_dCoh_lem", ``
-!s Icoh Icode Icm. cm_user_po Icoh Icode Icm /\ Icoh s ==> 
+!s Icoh Icode Icm. cm_user_po Icoh Icode Icm /\ Ifun s /\ Icoh s ==> 
     dCoh s.ms {pa | MEM pa IN CR s}
 ``,
   REWRITE_TAC [Icoh_dCoh_oblg]
@@ -76,7 +77,8 @@ val Icoh_dCoh_lem = store_thm("Icoh_dCoh_lem", ``
 
 val Icode_CR_lem = store_thm("Icode_CR_lem", ``
 !s s' Icoh Icode Icm. 
-       cm_user_po Icoh Icode Icm 
+       cm_user_po Icoh Icode Icm
+    /\ Ifun s
     /\ iCoh s.ms {pa | MEM pa IN CRex s}
     /\ iCoh s'.ms {pa | MEM pa IN CRex s'}
     /\ isafe s {pa | MEM pa IN CRex s}
@@ -89,14 +91,14 @@ val Icode_CR_lem = store_thm("Icode_CR_lem", ``
 );
 
 val Icode_iCoh_lem = store_thm("Icode_iCoh_lem", ``
-!s Icoh Icode Icm. cm_user_po Icoh Icode Icm /\ Icode s ==> 
+!s Icoh Icode Icm. cm_user_po Icoh Icode Icm /\ Ifun s /\ Icode s ==> 
     iCoh s.ms {pa | MEM pa IN CRex s}
 ``,
   REWRITE_TAC [Icode_iCoh_oblg]
 );
 
 val Icode_isafe_lem = store_thm("Icode_isafe_lem", ``
-!s Icoh Icode Icm. cm_user_po Icoh Icode Icm /\ Icode s ==> 
+!s Icoh Icode Icm. cm_user_po Icoh Icode Icm /\ Ifun s /\ Icode s ==> 
     isafe s {pa | MEM pa IN CRex s}
 ``,
   REWRITE_TAC [Icode_isafe_oblg]
@@ -353,7 +355,7 @@ val Inv_CR_unchanged_lem = store_thm("Inv_CR_unchanged_lem", ``
   STRIP_TAC
   >| [(* regs equal *)
       RW_TAC std_ss [Cv_reg_eq_def] >>
-      FULL_SIMP_TAC std_ss [drvbl_def] >>
+      FULL_SIMP_TAC std_ss [drvbl_def, Inv_lem] >>
       IMP_RES_TAC CR_coreg_lem >>
       ASM_REWRITE_TAC []
       ,
@@ -376,6 +378,7 @@ val Inv_CR_lem = store_thm("Inv_CR_lem", ``
 ``,
   REPEAT STRIP_TAC >>
   IMP_RES_TAC Inv_CR_unchanged_lem >>
+  FULL_SIMP_TAC std_ss [Inv_lem] >>
   IMP_RES_TAC CR_lem >>
   ASM_REWRITE_TAC []
 );
@@ -621,12 +624,12 @@ val Kcode_spec = new_specification ("Kcode_spec",
 
 val Ifun_AC_po = Define `Ifun_AC_po = 
 !s. Ifun s ==> 
-    !pa. pa IN Mac ==> only_CA s pa
+    (!pa. pa IN Mac ==> only_CA s pa)
+ /\ (!pa. MEM pa IN CR s ==> pa IN Mac)
 `;
 
 val Icoh_AC_def = Define `Icoh_AC s = 
-    (!pa. MEM pa IN CR s ==> pa IN Mac)
- /\ dCoh s.ms (Mac INTER {pa | MEM pa IN CR s})
+    dCoh s.ms (Mac INTER {pa | MEM pa IN CR s})
 `; 
 
 val Icode_AC_def = Define `Icode_AC s = 
@@ -666,6 +669,7 @@ val Inv_AC_CR_unchanged_lem = store_thm("Inv_AC_CR_unchanged_lem", ``
       `MEM pa IN CR s` by ( 
           FULL_SIMP_TAC std_ss [pred_setTheory.IN_GSPEC_IFF]
       ) >>
+      IMP_RES_TAC Ifun_AC_po >>
       FULL_SIMP_TAC std_ss []
      ]
 );
@@ -702,6 +706,7 @@ Ifun_AC_po ==> cm_user_po Icoh_AC Icode_AC Icm_AC
       `MEM pa IN CR s` by ( 
           FULL_SIMP_TAC std_ss [pred_setTheory.IN_GSPEC_IFF]
       ) >>
+      IMP_RES_TAC Ifun_AC_po >>
       FULL_SIMP_TAC std_ss []
       ,
       (* Icode_CR_po *)
@@ -849,18 +854,9 @@ val ca_Inv_rebuild_lem = store_thm("ca_Inv_rebuild_lem", ``
 ``,
   RW_TAC std_ss [cm_kernel_po_def] >>
   IMP_RES_TAC Icm_f_po_def >>
-  FULL_SIMP_TAC std_ss [ca_II_def, Inv_lem] >>
-  REPEAT STRIP_TAC
-  >| [(* Ifun *)
-      `Icoh sc'` by ( IMP_RES_TAC ca_Icmf_Icoh_lem ) >>
-      IMP_RES_TAC Ifun_Icoh_lem 
-      ,
-      (* Icoh *)
-      IMP_RES_TAC ca_Icmf_Icoh_lem
-      ,
-      (* Icode *)
-      IMP_RES_TAC ca_Icmf_Icode_lem 
-     ]
+  FULL_SIMP_TAC std_ss [Inv_lem, Inv_rebuild_po_def] >>
+  RES_TAC >>
+  ASM_REWRITE_TAC []
 );
 
 val kernel_bisim_lem = store_thm("kernel_bisim_lem", ``
